src/klas/Klas.Rot.fst
@@ -6,6 +6,9 @@ module Klas.Rot
 open Kuiper
 open Kuiper.Array1
 open Kuiper.Tensor.Layout.Alg { l1_forward }
+open Kuiper.Complex32
+open Kuiper.Complex64
+open Kuiper.Complex.Class { complex, of_real }
 module Map = Kuiper.Kernel.Map
 
 inline_for_extraction noextract
@@ -32,3 +35,28 @@ fn rot_gen (#et:Type0) {| floating et |}
 let rot_f16 = rot_gen #f16
 let rot_f32 = rot_gen #f32
 let rot_f64 = rot_gen #f64
+
+(* Csrot/Zdrot: real cosine/sine, complex vectors. See Klas.Rot.fsti. *)
+inline_for_extraction noextract
+fn csrot_gen (#c #r:Type0) {| scalar c |} {| floating r |} {| complex c r |}
+  (cc ss : r)
+  (lena : szp { lena <= max_blocks * max_threads })
+  (x : array1 c (l1_forward lena) { is_global x })
+  (y : array1 c (l1_forward lena) { is_global y })
+  (#vx : erased (lseq c lena))
+  (#vy : erased (lseq c lena))
+  preserves cpu
+  requires
+    on gpu_loc (x |-> vx) ** on gpu_loc (y |-> vy)
+  ensures
+    on gpu_loc (x |-> s_csrot_x cc ss vx vy) ** on gpu_loc (y |-> s_csrot_y cc ss vx vy)
+{
+  let tmp = alloc0 #c lena (l1_forward lena);
+  memcpy_device_to_device tmp x lena;
+  Map.map_gpu2 (fun (xi yi : c) -> add (mul (of_real cc) xi) (mul (of_real ss) yi)) lena x y;
+  Map.map_gpu2 (fun (yi ti : c) -> add (mul (of_real cc) yi) (mul (of_real (sub zero ss)) ti)) lena y tmp;
+  free tmp;
+}
+
+let csrot_cf32 = csrot_gen #cf32 #f32
+let csrot_cf64 = csrot_gen #cf64 #f64
